a lot of changes in the event system. first version of refinement relation

txn-data-consistency/CCv_Eiger_Port_modified.thy
@@ -24,9 +24,11 @@ definition ep_version_init :: "'v ep_version" where
     v_ts = 0, v_gst = 0, v_is_pending = False\<rparr>"
 
 \<comment> \<open>Server State\<close>
-datatype 'v state_wtxn = Ready | Prep tstmp 'v | Commit 'v
+datatype state_wtxn = Ready | Prep tstmp | Commit
+datatype state_rtxn = NotReg | Regd
 record 'v server =
-  wtxn_state :: "txid0 \<Rightarrow> key \<Rightarrow> 'v state_wtxn"
+  wtxn_state :: "txid0 \<Rightarrow> key \<Rightarrow> state_wtxn"
+  rtxn_state :: "txid0 \<Rightarrow> key \<Rightarrow> state_rtxn"
   clock :: tstmp
   lst :: tstmp
   pending_wtxns :: "txid0 \<rightharpoonup> tstmp"
@@ -43,6 +45,7 @@ record 'v client =
   txn_sn :: sqn
   gst :: tstmp
   lst_map :: "svr_id \<Rightarrow> tstmp"
+  cl_view :: view
 
 \<comment> \<open>Global State\<close>
 record 'v state = 
@@ -51,102 +54,157 @@ record 'v state =
 
 subsubsection \<open>Events\<close>
 
-datatype 'v ev = RInvoke cl_id "key set" | Read cl_id key 'v | RDone cl_id "key \<rightharpoonup> 'v" |
-  WInvoke cl_id "key \<rightharpoonup> 'v" | WriteAll cl_id "key \<rightharpoonup> 'v" tstmp | WDone cl_id |
-  WPrep svr_id txid0 key 'v | WCommit svr_id txid0 key | Skip2
+datatype 'v ev =
+  RInvoke cl_id "key set" sqn view "'v fingerpr"| Read cl_id key 'v | RDone cl_id "key \<rightharpoonup> 'v" |
+  WInvoke cl_id "key \<rightharpoonup> 'v" | WCommit cl_id "key \<rightharpoonup> 'v" tstmp sqn view "'v fingerpr" | WDone cl_id |
+  RegR svr_id txid0 key 'v v_id tstmp | PrepW svr_id txid0 key 'v tstmp | CommitW svr_id txid0 key |
+  Skip2
 
-fun at :: "'v ep_version list \<Rightarrow> tstmp \<Rightarrow> 'v ep_version" where
-  "at [] ts = ep_version_init" |
-  "at (ver # vl) ts = (if ts \<ge> v_ts ver then ver else at vl ts)"
+abbreviation get_txn_cl :: "'v state \<Rightarrow> cl_id \<Rightarrow> txid0" where
+  "get_txn_cl s cl \<equiv> Tn_cl (txn_sn (cls s cl)) cl"
 
-fun newest_own_write :: "'v ep_version list \<Rightarrow> tstmp \<Rightarrow> cl_id \<Rightarrow> 'v ep_version option" where
+(*Assumption: vl is ordered from the newest to the oldest*)
+fun at :: "'v ep_version list \<Rightarrow> tstmp \<Rightarrow> 'v ep_version \<times> v_id" where
+  "at [] ts = (ep_version_init, 0)" |
+  "at (ver # vl) ts = (if ts \<ge> v_ts ver then (ver, length vl) else at vl ts)"
+
+(*Assumption: vl is ordered from the newest to the oldest*)
+fun newest_own_write :: "'v ep_version list \<Rightarrow> tstmp \<Rightarrow> cl_id \<rightharpoonup> 'v ep_version \<times> v_id" where
   "newest_own_write [] ts cl = None" |
   "newest_own_write (v # vl) ts cl =
     (if v_ts v \<ge> ts then
       (case v_writer v of
         T0 \<Rightarrow> newest_own_write vl ts cl |
-        Tn (Tn_cl sn cl') \<Rightarrow> (if cl' = cl then Some v else newest_own_write vl ts cl))
+        Tn (Tn_cl sn cl') \<Rightarrow> (if cl' = cl then Some (v, length vl) else newest_own_write vl ts cl))
      else None)"
 
+(*Assumption: vl is ordered from the newest to the oldest*)
+definition read_at :: "'v ep_version list \<Rightarrow> tstmp \<Rightarrow> cl_id \<Rightarrow> 'v \<times> v_id" where
+  "read_at vl ts cl \<equiv> let (ver, i) = at vl ts in
+    (case newest_own_write vl (v_ts ver) cl of
+      None \<Rightarrow> (v_value ver, i) | Some (ver', i') \<Rightarrow> (v_value ver', i'))"
+
 \<comment> \<open>Clint Events\<close>
-definition read_invoke :: "cl_id \<Rightarrow> key set \<Rightarrow> 'v state \<Rightarrow> 'v state \<Rightarrow> bool" where
-  "read_invoke cl keys s s' \<equiv> 
+definition read_invoke :: "cl_id \<Rightarrow> key set \<Rightarrow> sqn \<Rightarrow> view \<Rightarrow> 'v fingerpr \<Rightarrow> 'v state \<Rightarrow> 'v state \<Rightarrow> bool" where
+  "read_invoke cl keys sn u F s s' \<equiv> 
+    sn = txn_sn (cls s cl) \<and>
+    u = cl_view (cls s cl) \<and>
+    (\<forall>k. F k W = None) \<and> (\<forall>k. k \<notin> keys \<longrightarrow> F k R = None) \<and>
+    (\<forall>k \<in> keys. \<exists>v i. F k R = Some v \<and>
+     (v, i) = read_at (rev (DS (svrs s (loc k)) k)) (gst (cls s cl)) cl \<and>
+     cl_view (cls s' cl) k = insert i (cl_view (cls s cl) k)) \<and>
     txn_state (cls s cl) = Idle \<and>
     txn_state (cls s' cl) = RtxnInProg keys (Map.empty) \<and>
     txn_sn (cls s' cl) = txn_sn (cls s cl) \<and>
     gst (cls s' cl) = max (gst (cls s cl)) (Min (range (lst_map (cls s cl)))) \<and>
     lst_map (cls s' cl) = lst_map (cls s cl) \<and>
+    (\<forall>k'. k' \<notin> keys \<longrightarrow> cl_view (cls s' cl)k' = cl_view (cls s cl) k') \<and>
     svrs s' = svrs s"
+
+fun find_and_read_val :: "'v ep_version list \<Rightarrow> txid0 \<rightharpoonup> 'v" where
+  "find_and_read_val [] t = None" |
+  "find_and_read_val (ver # vl) t =
+    (if t \<in> v_readerset ver then Some (v_value ver) else find_and_read_val vl t)"
 
 definition read :: "cl_id \<Rightarrow> key \<Rightarrow> 'v \<Rightarrow> 'v state \<Rightarrow> 'v state \<Rightarrow> bool" where
   "read cl k v s s' \<equiv> \<exists>keys vals.
+    rtxn_state (svrs s (loc k)) (get_txn_cl s cl) k = Regd \<and>
+    Some v = find_and_read_val (rev (DS (svrs s (loc k)) k)) (get_txn_cl s cl) \<and>
     txn_state (cls s cl) = RtxnInProg keys vals \<and> k \<in> keys \<and> vals k = None \<and>
     txn_state (cls s' cl) = RtxnInProg keys (vals (k \<mapsto> v)) \<and>
-    v = (let vl = (DS (svrs s (loc k)) k); ver = at vl (gst (cls s cl)) in
-      (case newest_own_write vl (v_ts ver) cl of None \<Rightarrow> v_value ver | Some ver' \<Rightarrow> v_value ver')) \<and>
     txn_sn (cls s' cl) = txn_sn (cls s cl) \<and>
     gst (cls s' cl) = gst (cls s cl) \<and>
     lst_map (cls s' cl) (loc k) = lst (svrs s (loc k)) \<and>
     (\<forall>l. l \<noteq> loc k \<longrightarrow> lst_map (cls s' cl) = lst_map (cls s cl)) \<and>
+    cl_view (cls s' cl) = cl_view (cls s cl) \<and>
     svrs s' = svrs s"
 
 definition read_done :: "cl_id \<Rightarrow> (key \<rightharpoonup> 'v) \<Rightarrow> 'v state \<Rightarrow> 'v state \<Rightarrow> bool" where
-  "read_done cl vals s s' \<equiv> \<exists>keys.
+  "read_done cl vals s s' \<equiv> (\<exists>keys.
     txn_state (cls s cl) = RtxnInProg keys vals \<and> dom vals = keys \<and>
+    (\<forall>k\<in>keys. rtxn_state (svrs s (loc k)) (get_txn_cl s cl) k = Regd)) \<and>
     txn_state (cls s' cl) = Idle \<and>
     txn_sn (cls s' cl) = Suc (txn_sn (cls s cl)) \<and>
     gst (cls s' cl) = gst (cls s cl) \<and>
     lst_map (cls s' cl) = lst_map (cls s cl) \<and>
+    cl_view (cls s' cl) = cl_view (cls s cl) \<and>
     svrs s' = svrs s"
 
 definition write_invoke :: "cl_id \<Rightarrow> (key \<rightharpoonup> 'v) \<Rightarrow> 'v state \<Rightarrow> 'v state \<Rightarrow> bool" where
   "write_invoke cl kv_map s s' \<equiv> 
+    kv_map \<noteq> Map.empty \<and>
     txn_state (cls s cl) = Idle \<and>
     txn_state (cls s' cl) = WtxnPrep kv_map \<and>
     txn_sn (cls s' cl) = txn_sn (cls s cl) \<and>
     gst (cls s' cl) = gst (cls s cl) \<and>
     lst_map (cls s' cl) = lst_map (cls s cl) \<and>
+    cl_view (cls s' cl) = cl_view (cls s cl) \<and>
     svrs s' = svrs s"
 
-definition write_all :: "cl_id \<Rightarrow> (key \<rightharpoonup> 'v) \<Rightarrow> tstmp \<Rightarrow> 'v state \<Rightarrow> 'v state \<Rightarrow> bool" where
-  "write_all cl kv_map commit_t s s' \<equiv>
+definition write_commit :: "cl_id \<Rightarrow> (key \<rightharpoonup> 'v) \<Rightarrow> tstmp \<Rightarrow> sqn \<Rightarrow> view \<Rightarrow> 'v fingerpr \<Rightarrow> 'v state \<Rightarrow> 'v state \<Rightarrow> bool" where
+  "write_commit cl kv_map commit_t sn u F s s' \<equiv>
+    sn = txn_sn (cls s cl) \<and>
+    u = cl_view (cls s cl) \<and>
+    (\<forall>k. F k R = None) \<and> (\<forall>k. F k W = kv_map k) \<and>
     txn_state (cls s cl) = WtxnPrep kv_map \<and>
-    (\<forall>k\<in>dom kv_map. \<exists>prep_t v.
-      wtxn_state (svrs s (loc k)) (Tn_cl (txn_sn (cls s cl)) cl) k = Prep prep_t v \<and> 
-      kv_map k = Some v \<and> prep_t \<le> commit_t) \<and>
+    (\<forall>k \<in> dom kv_map. \<exists>prep_t.
+      wtxn_state (svrs s (loc k)) (get_txn_cl s cl) k = Prep prep_t) \<and>
+    commit_t = Max {prep_t. (\<exists>k \<in> dom kv_map.
+      wtxn_state (svrs s (loc k)) (get_txn_cl s cl) k = Prep prep_t)} \<and>
     txn_state (cls s' cl) = WtxnCommit commit_t kv_map \<and>
     txn_sn (cls s' cl) = txn_sn (cls s cl) \<and>
     gst (cls s' cl) = gst (cls s cl) \<and>
     lst_map (cls s' cl) = lst_map (cls s cl) \<and>
+    \<comment> \<open>update cl_view\<close>
     svrs s' = svrs s"
 
 definition write_done :: "cl_id \<Rightarrow> 'v state \<Rightarrow> 'v state \<Rightarrow> bool" where
   "write_done cl s s' \<equiv> \<exists>kv_map commit_t.
     txn_state (cls s cl) = WtxnCommit commit_t kv_map \<and>
-    (\<forall>k\<in>dom kv_map. \<exists>v. wtxn_state (svrs s (loc k)) (Tn_cl (txn_sn (cls s cl)) cl) k = Commit v \<and>
-       kv_map k = Some v) \<and>
+    (\<forall>k\<in>dom kv_map. wtxn_state (svrs s (loc k)) (get_txn_cl s cl) k = Commit) \<and>
     txn_state (cls s' cl) = Idle \<and>
     txn_sn (cls s' cl) = Suc (txn_sn (cls s cl)) \<and>
     gst (cls s' cl) = gst (cls s cl) \<and>
     (\<forall>l. l \<in> loc ` (dom kv_map) \<longrightarrow> lst_map (cls s' cl) l = lst (svrs s l)) \<and>
     (\<forall>l. l \<notin> loc ` (dom kv_map) \<longrightarrow> lst_map (cls s' cl) l = lst_map (cls s cl) l) \<and>
+    cl_view (cls s' cl) = cl_view (cls s cl) \<and>
     svrs s' = svrs s"
 
 \<comment> \<open>Server Events\<close>
-definition prepare_write :: "svr_id \<Rightarrow> txid0 \<Rightarrow> key \<Rightarrow> 'v \<Rightarrow> 'v state \<Rightarrow> 'v state \<Rightarrow> bool" where
-  "prepare_write svr t k v s s' \<equiv> \<exists>kv_map.
-    txn_state (cls s (get_cl_txn t)) = WtxnPrep kv_map \<and> k \<in> dom kv_map \<and> kv_map k = Some v \<and>
-    wtxn_state (svrs s svr) t k = Ready \<and>
-    wtxn_state (svrs s' svr) t k = Prep (clock (svrs s' svr)) v \<and>
-    (\<forall>t' k'. t' \<noteq> t \<or> k' \<noteq> k \<longrightarrow> wtxn_state (svrs s' svr) t' = wtxn_state (svrs s svr) t') \<and>
+definition register_read :: "svr_id \<Rightarrow> txid0 \<Rightarrow> key \<Rightarrow> 'v \<Rightarrow> v_id \<Rightarrow> tstmp \<Rightarrow> 'v state \<Rightarrow> 'v state \<Rightarrow> bool" where
+  "register_read svr t k v i gst_ts s s' \<equiv> \<exists>keys vals.
+    txn_state (cls s (get_cl_txn t)) = RtxnInProg keys vals \<and> k \<in> keys \<and> vals k = None \<and>
+    (v, i) = read_at (rev (DS (svrs s svr) k)) gst_ts (get_cl_txn t) \<and>
+    gst_ts = gst (cls s (get_cl_txn t)) \<and>
     loc k = svr \<and>
+    rtxn_state (svrs s svr) t k = NotReg \<and>
+    rtxn_state (svrs s' svr) t k = Regd \<and>
+    (\<forall>t' k'. t' \<noteq> t \<or> k' \<noteq> k \<longrightarrow> rtxn_state (svrs s' svr) t' k' = rtxn_state (svrs s svr) t' k') \<and>
+    wtxn_state (svrs s' svr) = wtxn_state (svrs s svr) \<and>
+    clock (svrs s' svr) = Suc (clock (svrs s svr)) \<and>
+    lst (svrs s' svr) = lst (svrs s svr) \<and>
+    pending_wtxns (svrs s' svr) = pending_wtxns (svrs s svr) \<and>
+    DS (svrs s' svr) k = (DS (svrs s svr) k) [i :=
+      (DS (svrs s svr) k ! i)\<lparr>v_readerset := insert t (v_readerset (DS (svrs s svr) k ! i))\<rparr>] \<and>
+    (\<forall>k'. k' \<noteq> k \<longrightarrow> DS (svrs s' svr) k' = DS (svrs s svr) k') \<and>
+    cls s' = cls s"
+
+definition prepare_write :: "svr_id \<Rightarrow> txid0 \<Rightarrow> key \<Rightarrow> 'v \<Rightarrow> tstmp \<Rightarrow> 'v state \<Rightarrow> 'v state \<Rightarrow> bool" where
+  "prepare_write svr t k v gst_ts s s' \<equiv> \<exists>kv_map.
+    txn_state (cls s (get_cl_txn t)) = WtxnPrep kv_map \<and> k \<in> dom kv_map \<and> kv_map k = Some v \<and>
+    gst_ts =  (gst (cls s (get_cl_txn t))) \<and> 
+    loc k = svr \<and>
+    wtxn_state (svrs s svr) t k = Ready \<and>
+    wtxn_state (svrs s' svr) t k = Prep (clock (svrs s' svr)) \<and>
+    (\<forall>t' k'. t' \<noteq> t \<or> k' \<noteq> k \<longrightarrow> wtxn_state (svrs s' svr) t' k' = wtxn_state (svrs s svr) t' k') \<and>
+    rtxn_state (svrs s' svr) = rtxn_state (svrs s svr) \<and>
     clock (svrs s' svr) = Suc (clock (svrs s svr)) \<and>
     lst (svrs s' svr) = lst (svrs s svr) \<and>
     pending_wtxns (svrs s' svr) t = Some (clock (svrs s svr)) \<and>
     (\<forall>t'. t' \<noteq> t \<longrightarrow> pending_wtxns (svrs s' svr) t' = pending_wtxns (svrs s svr) t') \<and>
-    DS (svrs s' svr) k =
-      \<lparr>v_value = v, v_writer = Tn t, v_readerset = {}, v_ts = clock (svrs s svr),
-       v_gst = (gst (cls s (get_cl_txn t))), v_is_pending = True\<rparr> # DS (svrs s svr) k \<and>
+    DS (svrs s' svr) k = DS (svrs s svr) k @
+      [\<lparr>v_value = v, v_writer = Tn t, v_readerset = {}, v_ts = clock (svrs s svr),
+       v_gst = gst_ts, v_is_pending = True\<rparr>] \<and>
     (\<forall>k'. k' \<noteq> k \<longrightarrow> DS (svrs s' svr) k' = DS (svrs s svr) k') \<and>
     cls s' = cls s"
 
@@ -160,10 +218,11 @@ fun find_and_commit :: "'v ep_version list \<Rightarrow> txid \<Rightarrow> tstm
 definition commit_write :: "svr_id \<Rightarrow> txid0 \<Rightarrow> key \<Rightarrow> 'v state \<Rightarrow> 'v state \<Rightarrow> bool" where
   "commit_write svr t k s s' \<equiv> \<exists>kv_map commit_t.
     txn_state (cls s (get_cl_txn t)) = WtxnCommit commit_t kv_map \<and> k \<in> dom kv_map \<and>
-    (\<exists>prep_t v. wtxn_state (svrs s svr) t k = Prep prep_t v \<and> kv_map k = Some v \<and>
-      wtxn_state (svrs s' svr) t k = Commit v) \<and>
-    (\<forall>t' k'. t' \<noteq> t \<or> k' \<noteq> k \<longrightarrow> pending_wtxns (svrs s' svr) t' = pending_wtxns (svrs s svr) t') \<and>
     loc k = svr \<and>
+    (\<exists>prep_t. wtxn_state (svrs s svr) t k = Prep prep_t) \<and>
+    wtxn_state (svrs s' svr) t k = Commit \<and>
+    (\<forall>t' k'. t' \<noteq> t \<or> k' \<noteq> k \<longrightarrow> wtxn_state (svrs s' svr) t' k' = wtxn_state (svrs s svr) t' k) \<and>
+    rtxn_state (svrs s' svr) = rtxn_state (svrs s svr) \<and>
     clock (svrs s' svr) = clock (svrs s svr) \<and>
     lst (svrs s' svr) =
       (if dom (pending_wtxns (svrs s' svr)) = {} then clock (svrs s svr)
@@ -180,8 +239,10 @@ definition state_init :: "'v state" where
     cls = (\<lambda>cl. \<lparr> txn_state = Idle,
                   txn_sn = 0,
                   gst = 0,
-                  lst_map = (\<lambda>svr. 0) \<rparr>),
+                  lst_map = (\<lambda>svr. 0),
+                  cl_view = view_init \<rparr>),
     svrs = (\<lambda>svr. \<lparr> wtxn_state = (\<lambda>t k. Ready),
+                    rtxn_state = (\<lambda>t k. NotReg),
                     clock = 0,
                     lst = 0,
                     pending_wtxns = Map.empty,
@@ -189,14 +250,15 @@ definition state_init :: "'v state" where
   \<rparr>"
 
 fun state_trans :: "'v state \<Rightarrow> 'v ev \<Rightarrow> 'v state \<Rightarrow> bool" where
-  "state_trans s (RInvoke cl keys)        s' \<longleftrightarrow> read_invoke cl keys s s'" |
+  "state_trans s (RInvoke cl keys sn u F) s' \<longleftrightarrow> read_invoke cl keys sn u F s s'" |
   "state_trans s (Read cl k v)            s' \<longleftrightarrow> read cl k v s s'" |
   "state_trans s (RDone cl kv_map)        s' \<longleftrightarrow> read_done cl kv_map s s'" |
   "state_trans s (WInvoke cl kv_map)      s' \<longleftrightarrow> write_invoke cl kv_map s s'" |
-  "state_trans s (WriteAll cl kv_map cts) s' \<longleftrightarrow> write_all cl kv_map cts s s'" |
+  "state_trans s (WCommit cl kv_map cts sn u F)  s' \<longleftrightarrow> write_commit cl kv_map cts sn u F s s'" |
   "state_trans s (WDone cl)               s' \<longleftrightarrow> write_done cl s s'" |
-  "state_trans s (WPrep svr t k v)        s' \<longleftrightarrow> prepare_write svr t k v s s'" |
-  "state_trans s (WCommit svr t k)        s' \<longleftrightarrow> commit_write svr t k s s'" |
+  "state_trans s (RegR svr t k v i gts)   s' \<longleftrightarrow> register_read svr t k v i gts s s'" |
+  "state_trans s (PrepW svr t k v gts)    s' \<longleftrightarrow> prepare_write svr t k v gts s s'" |
+  "state_trans s (CommitW svr t k)        s' \<longleftrightarrow> commit_write svr t k s s'" |
   "state_trans s Skip2 s' \<longleftrightarrow> s' = s"
 
 definition tps :: "('v ev, 'v state) ES" where
@@ -205,9 +267,36 @@ definition tps :: "('v ev, 'v state) ES" where
     trans = state_trans
   \<rparr>"
 
-lemmas tps_trans_defs = read_invoke_def read_def read_done_def write_invoke_def write_all_def
-  write_done_def prepare_write_def commit_write_def
+lemmas tps_trans_defs = read_invoke_def read_def read_done_def write_invoke_def write_commit_def
+  write_done_def register_read_def prepare_write_def commit_write_def
 
 lemmas tps_defs = tps_def state_init_def
 
 lemma tps_trans [simp]: "trans tps = state_trans" by (simp add: tps_def)
+
+subsubsection \<open>Refinement\<close>
+
+\<comment> \<open>Simulation function\<close>
+definition get_ver :: "'v ep_version \<Rightarrow> 'v version" where
+  "get_ver v \<equiv> \<lparr>v_value = v_value v, v_writer = v_writer v, v_readerset = v_readerset v\<rparr>"
+
+\<comment> \<open>TODO: define this properly\<close>
+definition kvs_of_s :: "'v state \<Rightarrow> 'v kv_store" where
+  "kvs_of_s s = (\<lambda>k. map get_ver (DS (svrs s (loc k)) k))"
+
+definition views_of_s :: "'v state \<Rightarrow> (cl_id \<Rightarrow> view)" where
+  "views_of_s s = (\<lambda>cl. cl_view (cls s cl))"
+
+definition sim :: "'v state \<Rightarrow> 'v config" where         
+  "sim s = (kvs_of_s s, views_of_s s)"
+
+(*lemmas update_kv_reads_all_defs = update_kv_reads_all_txn_def Let_def last_version_def
+lemmas update_kv_all_defs = update_kv_reads_all_defs update_kv_writes_all_txn_def update_kv_all_txn_def*)
+lemmas sim_defs = sim_def kvs_of_s_def views_of_s_def
+
+\<comment> \<open>Mediator function\<close>
+fun med :: "'v ev \<Rightarrow> 'v label" where
+  "med (RInvoke cl _ sn u F) = ET cl sn u F" |
+  "med (WCommit cl _ _ sn u F) = ET cl sn u F" |
+  "med _ = ETSkip"
+
